lib/Monads/nondet/Nondet_Sat.thy
@@ -17,7 +17,8 @@ text \<open>
   The dual to validity: an existential instead of a universal quantifier for the post condition.
   In refinement, it is often sufficient to know that there is one state that satisfies a condition.\<close>
 definition exs_valid ::
-  "('a \<Rightarrow> bool) \<Rightarrow> ('a, 'b) nondet_monad \<Rightarrow> ('b \<Rightarrow> 'a \<Rightarrow> bool) \<Rightarrow> bool" ("\<lbrace>_\<rbrace> _ \<exists>\<lbrace>_\<rbrace>") where
+  "('a \<Rightarrow> bool) \<Rightarrow> ('a, 'b) nondet_monad \<Rightarrow> ('b \<Rightarrow> 'a \<Rightarrow> bool) \<Rightarrow> bool"
+  ("\<lbrace>_\<rbrace> _ \<exists>\<lbrace>_\<rbrace>") where
   "\<lbrace>P\<rbrace> f \<exists>\<lbrace>Q\<rbrace> \<equiv> \<forall>s. P s \<longrightarrow> (\<exists>(rv, s') \<in> fst (f s). Q rv s')"
 
 text \<open>The above for the exception monad\<close>
