lib/Monads/trace/Trace_Monad.thy
@@ -38,13 +38,12 @@ datatype ('s, 'a) tmres = Failed | Incomplete | Result "('a \<times> 's)"
 abbreviation map_tmres_rv :: "('a \<Rightarrow> 'b) \<Rightarrow> ('s, 'a) tmres \<Rightarrow> ('s, 'b) tmres" where
   "map_tmres_rv f \<equiv> map_tmres id f"
 
-section "The Monad"
-
 text \<open>
   tmonad returns a set of non-deterministic computations, including
   a trace as a list of "thread identifier" \<times> state, and an optional
   pair of result and state when the computation did not fail.\<close>
 type_synonym ('s, 'a) tmonad = "'s \<Rightarrow> ((tmid \<times> 's) list \<times> ('s, 'a) tmres) set"
+
 
 text \<open>
   Print the type @{typ "('s,'a) tmonad"} instead of its unwieldy expansion.
@@ -63,6 +62,7 @@ print_ast_translation \<open>
       then Ast.Appl [Ast.Constant @{type_syntax "tmonad"}, t1, t4]
       else raise Match
   in [(@{type_syntax "fun"}, tmonad_tr)] end\<close>
+
 
 text \<open>Returns monad results, ignoring failures and traces.\<close>
 definition mres :: "((tmid \<times> 's) list \<times> ('s, 'a) tmres) set \<Rightarrow> ('a \<times> 's) set" where
@@ -98,7 +98,7 @@ definition bind ::
     | Result (rv, s) \<Rightarrow> fst_upd (\<lambda>ys. ys @ xs) ` g rv s"
 
 text \<open>Sometimes it is convenient to write @{text bind} in reverse order.\<close>
-abbreviation(input) bind_rev ::
+abbreviation (input) bind_rev ::
   "('c \<Rightarrow> ('a, 'b) tmonad) \<Rightarrow> ('a, 'c) tmonad \<Rightarrow> ('a, 'b) tmonad" (infixl "=<<" 60)
   where
   "g =<< f \<equiv> f >>= g"
@@ -123,6 +123,7 @@ primrec put_trace :: "(tmid \<times> 's) list \<Rightarrow> ('s, unit) tmonad" w
     "put_trace [] = return ()"
   | "put_trace (x # xs) = (put_trace xs >>= (\<lambda>_. put_trace_elem x))"
 
+
 subsection "Nondeterminism"
 
 text \<open>
@@ -134,8 +135,9 @@ text \<open>
 definition select :: "'a set \<Rightarrow> ('s, 'a) tmonad" where
   "select A \<equiv> \<lambda>s. (Pair [] ` Result ` (A \<times> {s}))"
 
-definition alternative :: "('s,'a) tmonad \<Rightarrow> ('s,'a) tmonad \<Rightarrow> ('s,'a) tmonad"
-  (infixl "\<sqinter>" 20) where
+definition alternative ::
+  "('s,'a) tmonad \<Rightarrow> ('s,'a) tmonad \<Rightarrow> ('s,'a) tmonad" (infixl "\<sqinter>" 20)
+  where
   "f \<sqinter> g \<equiv> \<lambda>s. (f s \<union> g s)"
 
 text \<open>
@@ -152,6 +154,7 @@ text \<open>
 definition state_select :: "('s \<times> 's) set \<Rightarrow> ('s, unit) tmonad" where
   "state_select r \<equiv>
      \<lambda>s. (Pair [] ` default_elem Failed (Result ` (\<lambda>x. ((), x)) ` {s'. (s, s') \<in> r}))"
+
 
 subsection "Failure"
 
@@ -202,7 +205,8 @@ text \<open>
   Perform a test on the current state, performing the left monad if
   the result is true or the right monad if the result is false.\<close>
 definition condition ::
-  "('s \<Rightarrow> bool) \<Rightarrow> ('s, 'r) tmonad \<Rightarrow> ('s, 'r) tmonad \<Rightarrow> ('s, 'r) tmonad" where
+  "('s \<Rightarrow> bool) \<Rightarrow> ('s, 'r) tmonad \<Rightarrow> ('s, 'r) tmonad \<Rightarrow> ('s, 'r) tmonad"
+  where
   "condition P L R \<equiv> \<lambda>s. if (P s) then (L s) else (R s)"
 
 notation (output)
@@ -217,15 +221,14 @@ definition gets_the :: "('s \<Rightarrow> 'a option) \<Rightarrow> ('s, 'a) tmon
 text \<open>
   Get a map (such as a heap) from the current state and apply an argument to the map.
   Fail if the map returns @{const None}, otherwise return the value.\<close>
-definition
-  gets_map :: "('s \<Rightarrow> 'a \<Rightarrow> 'b option) \<Rightarrow> 'a \<Rightarrow> ('s, 'b) tmonad" where
+definition gets_map :: "('s \<Rightarrow> 'a \<Rightarrow> 'b option) \<Rightarrow> 'a \<Rightarrow> ('s, 'b) tmonad" where
   "gets_map f p \<equiv> gets f >>= (\<lambda>m. assert_opt (m p))"
 
 
 subsection \<open>The Monad Laws\<close>
 
-text \<open>An alternative definition of bind, sometimes more convenient.\<close>
-lemma bind_def2:
+text \<open>An alternative definition of @{term bind}, sometimes more convenient.\<close>
+lemma bind_def':
   "bind f g \<equiv>
      \<lambda>s. ((\<lambda>xs. (xs, Failed)) ` {xs. (xs, Failed) \<in> f s})
          \<union> ((\<lambda>xs. (xs, Incomplete)) ` {xs. (xs, Incomplete) \<in> f s})
@@ -242,7 +245,7 @@ lemma elem_bindE:
     \<lbrakk>res = Incomplete \<or> res = Failed; (tr, map_tmres undefined undefined res) \<in> f s\<rbrakk> \<Longrightarrow> P;
     \<And>tr' tr'' x s'. \<lbrakk>(tr', Result (x, s')) \<in> f s; (tr'', res) \<in> g x s'; tr = tr'' @ tr'\<rbrakk> \<Longrightarrow> P\<rbrakk>
    \<Longrightarrow> P"
-  by (auto simp: bind_def2)
+  by (auto simp: bind_def')
 
 text \<open>Each monad satisfies at least the following three laws.\<close>
 
@@ -276,6 +279,7 @@ lemma bind_assoc:
   apply (split tmres.split; intro conjI impI; clarsimp)
   apply (simp add: image_image)
   done
+
 
 section \<open>Adding Exceptions\<close>
 
@@ -312,8 +316,8 @@ text \<open>
   the right-hand side is skipped if the left-hand side
   produced an exception.\<close>
 definition bindE ::
-  "('s, 'e + 'a) tmonad \<Rightarrow> ('a \<Rightarrow> ('s, 'e + 'b) tmonad) \<Rightarrow> ('s, 'e + 'b) tmonad"
-  (infixl ">>=E" 60) where
+  "('s, 'e + 'a) tmonad \<Rightarrow> ('a \<Rightarrow> ('s, 'e + 'b) tmonad) \<Rightarrow> ('s, 'e + 'b) tmonad" (infixl ">>=E" 60)
+  where
   "f >>=E g \<equiv> f >>= lift g"
 
 text \<open>
@@ -344,6 +348,7 @@ text \<open>
   instead of @{term return}.\<close>
 definition assertE :: "bool \<Rightarrow> ('a, 'e + unit) tmonad" where
   "assertE P \<equiv> if P then returnOk () else fail"
+
 
 subsection "Monad Laws for the Exception Monad"
 
@@ -545,7 +550,8 @@ text \<open>
   going through both lists simultaneously, left to right, ignoring
   return values.\<close>
 definition zipWithM_x ::
-  "('a \<Rightarrow> 'b \<Rightarrow> ('s,'c) tmonad) \<Rightarrow> 'a list \<Rightarrow> 'b list \<Rightarrow> ('s, unit) tmonad" where
+  "('a \<Rightarrow> 'b \<Rightarrow> ('s,'c) tmonad) \<Rightarrow> 'a list \<Rightarrow> 'b list \<Rightarrow> ('s, unit) tmonad"
+  where
   "zipWithM_x f xs ys \<equiv> sequence_x (zipWith f xs ys)"
 
 text \<open>
@@ -559,14 +565,16 @@ definition mapM :: "('a \<Rightarrow> ('s,'b) tmonad) \<Rightarrow> 'a list \<Ri
   "mapM f xs \<equiv> sequence (map f xs)"
 
 definition zipWithM ::
-  "('a \<Rightarrow> 'b \<Rightarrow> ('s,'c) tmonad) \<Rightarrow> 'a list \<Rightarrow> 'b list \<Rightarrow> ('s, 'c list) tmonad" where
+  "('a \<Rightarrow> 'b \<Rightarrow> ('s,'c) tmonad) \<Rightarrow> 'a list \<Rightarrow> 'b list \<Rightarrow> ('s, 'c list) tmonad"
+  where
   "zipWithM f xs ys \<equiv> sequence (zipWith f xs ys)"
 
 definition foldM :: "('b \<Rightarrow> 'a \<Rightarrow> ('s, 'a) tmonad) \<Rightarrow> 'b list \<Rightarrow> 'a \<Rightarrow> ('s, 'a) tmonad" where
   "foldM m xs a \<equiv> foldr (\<lambda>p q. q >>= m p) xs (return a) "
 
 definition foldME ::
-  "('b \<Rightarrow> 'a \<Rightarrow> ('s,('e + 'b)) tmonad) \<Rightarrow> 'b \<Rightarrow> 'a list \<Rightarrow> ('s, ('e + 'b)) tmonad" where
+  "('b \<Rightarrow> 'a \<Rightarrow> ('s,('e + 'b)) tmonad) \<Rightarrow> 'b \<Rightarrow> 'a list \<Rightarrow> ('s, ('e + 'b)) tmonad"
+  where
   "foldME m a xs \<equiv> foldr (\<lambda>p q. q >>=E swp m p) xs (returnOk a)"
 
 text \<open>
@@ -584,7 +592,6 @@ definition sequenceE :: "('s, 'e+'a) tmonad list \<Rightarrow> ('s, 'e+'a list) 
 
 definition mapME :: "('a \<Rightarrow> ('s,'e+'b) tmonad) \<Rightarrow> 'a list \<Rightarrow> ('s,'e+'b list) tmonad" where
   "mapME f xs \<equiv> sequenceE (map f xs)"
-
 
 text \<open>Filtering a list using a monadic function as predicate:\<close>
 primrec filterM :: "('a \<Rightarrow> ('s, bool) tmonad) \<Rightarrow> 'a list \<Rightarrow> ('s, 'a list) tmonad" where
@@ -617,7 +624,8 @@ text \<open>
   Turning an exception monad into a normal state monad
   by catching and handling any potential exceptions:\<close>
 definition catch ::
-  "('s, 'e + 'a) tmonad \<Rightarrow> ('e \<Rightarrow> ('s, 'a) tmonad) \<Rightarrow> ('s, 'a) tmonad" (infix "<catch>" 10) where
+  "('s, 'e + 'a) tmonad \<Rightarrow> ('e \<Rightarrow> ('s, 'a) tmonad) \<Rightarrow> ('s, 'a) tmonad" (infix "<catch>" 10)
+  where
   "f <catch> handler \<equiv>
      do x \<leftarrow> f;
         case x of
@@ -645,8 +653,8 @@ text \<open>
   practice: the exception handle (potentially) throws exception
   of the same type as the left-hand side.\<close>
 definition handleE ::
-  "('s, 'x + 'a) tmonad \<Rightarrow> ('x \<Rightarrow> ('s, 'x + 'a) tmonad) \<Rightarrow> ('s, 'x + 'a) tmonad"
-  (infix "<handle>" 10) where
+  "('s, 'x + 'a) tmonad \<Rightarrow> ('x \<Rightarrow> ('s, 'x + 'a) tmonad) \<Rightarrow> ('s, 'x + 'a) tmonad" (infix "<handle>" 10)
+  where
   "handleE \<equiv> handleE'"
 
 text \<open>
@@ -654,8 +662,8 @@ text \<open>
   if the left-hand side throws no exception:\<close>
 definition handle_elseE ::
   "('s, 'e + 'a) tmonad \<Rightarrow> ('e \<Rightarrow> ('s, 'ee + 'b) tmonad) \<Rightarrow> ('a \<Rightarrow> ('s, 'ee + 'b) tmonad) \<Rightarrow>
-   ('s, 'ee + 'b) tmonad"
-  ("_ <handle> _ <else> _" 10) where
+   ('s, 'ee + 'b) tmonad" ("_ <handle> _ <else> _" 10)
+  where
   "f <handle> handler <else> continue \<equiv>
    do v \<leftarrow> f;
    case v of Inl e  \<Rightarrow> handler e
@@ -698,7 +706,8 @@ inductive_cases whileLoop_terminates_cases: "whileLoop_terminates C B r s"
 inductive_simps whileLoop_terminates_simps: "whileLoop_terminates C B r s"
 
 definition whileLoop ::
-  "('r \<Rightarrow> 's \<Rightarrow> bool) \<Rightarrow> ('r \<Rightarrow> ('s, 'r) tmonad) \<Rightarrow> 'r \<Rightarrow> ('s, 'r) tmonad" where
+  "('r \<Rightarrow> 's \<Rightarrow> bool) \<Rightarrow> ('r \<Rightarrow> ('s, 'r) tmonad) \<Rightarrow> 'r \<Rightarrow> ('s, 'r) tmonad"
+  where
   "whileLoop C B \<equiv> (\<lambda>r s. {(ts, res). ((r,s), ts,res) \<in> whileLoop_results C B})"
 
 notation (output)
@@ -706,7 +715,8 @@ notation (output)
 
 \<comment> \<open>FIXME: why does this differ to Nondet_Monad?\<close>
 definition whileLoopT ::
-  "('r \<Rightarrow> 's \<Rightarrow> bool) \<Rightarrow> ('r \<Rightarrow> ('s, 'r) tmonad) \<Rightarrow> 'r \<Rightarrow> ('s, 'r) tmonad" where
+  "('r \<Rightarrow> 's \<Rightarrow> bool) \<Rightarrow> ('r \<Rightarrow> ('s, 'r) tmonad) \<Rightarrow> 'r \<Rightarrow> ('s, 'r) tmonad"
+  where
   "whileLoopT C B \<equiv> (\<lambda>r s. {(ts, res). ((r,s), ts,res) \<in> whileLoop_results C B
                                          \<and> whileLoop_terminates C B r s})"
 
@@ -714,7 +724,8 @@ notation (output)
   whileLoopT  ("(whileLoopT (_)//  (_))" [1000, 1000] 1000)
 
 definition whileLoopE ::
-  "('r \<Rightarrow> 's \<Rightarrow> bool) \<Rightarrow> ('r \<Rightarrow> ('s, 'e + 'r) tmonad) \<Rightarrow> 'r \<Rightarrow> ('s, ('e + 'r)) tmonad" where
+  "('r \<Rightarrow> 's \<Rightarrow> bool) \<Rightarrow> ('r \<Rightarrow> ('s, 'e + 'r) tmonad) \<Rightarrow> 'r \<Rightarrow> ('s, ('e + 'r)) tmonad"
+  where
   "whileLoopE C body \<equiv>
       \<lambda>r. whileLoop (\<lambda>r s. (case r of Inr v \<Rightarrow> C v s | _ \<Rightarrow> False)) (lift body) (Inr r)"
 
@@ -727,44 +738,38 @@ section "Combinators that have conditions with side effects"
 definition notM :: "('s, bool) tmonad \<Rightarrow> ('s, bool) tmonad" where
   "notM m = do c \<leftarrow> m; return (\<not> c) od"
 
-definition whileM ::
-  "('s, bool) tmonad \<Rightarrow> ('s, 'a) tmonad \<Rightarrow> ('s, unit) tmonad" where
+definition whileM :: "('s, bool) tmonad \<Rightarrow> ('s, 'a) tmonad \<Rightarrow> ('s, unit) tmonad" where
   "whileM C B \<equiv> do
     c \<leftarrow> C;
     whileLoop (\<lambda>c s. c) (\<lambda>_. do B; C od) c;
     return ()
   od"
 
-definition ifM ::
-  "('s, bool) tmonad \<Rightarrow> ('s, 'a) tmonad \<Rightarrow> ('s, 'a) tmonad \<Rightarrow>
-          ('s, 'a) tmonad" where
+definition ifM :: "('s, bool) tmonad \<Rightarrow> ('s, 'a) tmonad \<Rightarrow> ('s, 'a) tmonad \<Rightarrow> ('s, 'a) tmonad" where
   "ifM test t f = do
     c \<leftarrow> test;
     if c then t else f
    od"
 
 definition ifME ::
-  "('a, 'b + bool) tmonad \<Rightarrow> ('a, 'b + 'c) tmonad \<Rightarrow> ('a, 'b + 'c) tmonad
-   \<Rightarrow> ('a, 'b + 'c) tmonad" where
+  "('a, 'b + bool) tmonad \<Rightarrow> ('a, 'b + 'c) tmonad \<Rightarrow> ('a, 'b + 'c) tmonad \<Rightarrow> ('a, 'b + 'c) tmonad"
+  where
   "ifME test t f = doE
     c \<leftarrow> test;
     if c then t else f
    odE"
 
-definition whenM ::
-  "('s, bool) tmonad \<Rightarrow> ('s, unit) tmonad \<Rightarrow> ('s, unit) tmonad" where
+definition whenM :: "('s, bool) tmonad \<Rightarrow> ('s, unit) tmonad \<Rightarrow> ('s, unit) tmonad" where
   "whenM t m = ifM t m (return ())"
 
-definition orM ::
-  "('s, bool) tmonad \<Rightarrow> ('s, bool) tmonad \<Rightarrow> ('s, bool) tmonad" where
+definition orM :: "('s, bool) tmonad \<Rightarrow> ('s, bool) tmonad \<Rightarrow> ('s, bool) tmonad" where
   "orM a b = ifM a (return True) b"
 
-definition
-  andM :: "('s, bool) tmonad \<Rightarrow> ('s, bool) tmonad \<Rightarrow> ('s, bool) tmonad" where
+definition andM :: "('s, bool) tmonad \<Rightarrow> ('s, bool) tmonad \<Rightarrow> ('s, bool) tmonad" where
   "andM a b = ifM a b (return False)"
 
 
-subsection "Await command"
+section "Await command"
 
 text \<open>@{term "Await c f"} blocks the execution until @{term "c"} is true,
       and then atomically executes @{term "f"}.\<close>
@@ -782,7 +787,7 @@ definition Await :: "('s \<Rightarrow> bool) \<Rightarrow> ('s,unit) tmonad" whe
   od"
 
 
-section "Trace monad Parallel"
+section "Parallel combinator"
 
 definition parallel :: "('s,'a) tmonad \<Rightarrow> ('s,'a) tmonad \<Rightarrow> ('s,'a) tmonad" where
   "parallel f g = (\<lambda>s. {(xs, rv). \<exists>f_steps. length f_steps = length xs
