lib/Monads/trace/Trace_Monad_Equations.thy
@@ -286,6 +286,14 @@ lemma gets_fold_into_modify:
   by (simp_all add: fun_eq_iff modify_def bind_assoc exec_gets
                     exec_get exec_put)
 
+lemma gets_return_gets_eq:
+  "gets f >>= (\<lambda>g. return (h g)) = gets (\<lambda>s. h (f s))"
+  by (simp add: simpler_gets_def bind_def return_def)
+
+lemma gets_prod_comp:
+  "gets (case x of (a, b) \<Rightarrow> f a b) = (case x of (a, b) \<Rightarrow> gets (f a b))"
+  by (auto simp: split_def)
+
 lemma bind_assoc2:
   "(do x \<leftarrow> a; _ \<leftarrow> b; c x od) = (do x \<leftarrow> (do x' \<leftarrow> a; _ \<leftarrow> b; return x' od); c x od)"
   by (simp add: bind_assoc)
